thys/Real_Time_Deque/RealTimeDeque.thy
@@ -15,18 +15,18 @@ The real-time deque can be in the following states:
    \<^item> 3 * size of left end \<open>\<ge>\<close> size of right end
    \<^item> 3 * size of right end \<open>\<ge>\<close> size of left end
    \<^item> Neither of the ends is empty
- \<^descr> \<open>Transforming\<close>: Deque which violated the invariant of the \<open>idle\<close> state by non-balanced dequeue and enqueue operations. The invariants during in this state are:
-   \<^item> The transformation is not done yet. The deque needs to be in \<open>idle\<close> state otherwise.
-   \<^item> The transformation is in a valid state (Defined in theory \<open>States\<close>)
-   \<^item> The two ends of the deque are in a size window, such that after finishing the transformation the invariant of the \<open>idle\<close> state will be met. 
+ \<^descr> \<open>Rebal\<close>: Deque which violated the invariant of the \<open>idle\<close> state by non-balanced dequeue and enqueue operations. The invariants during in this state are:
+   \<^item> The rebalancing is not done yet. The deque needs to be in \<open>idle\<close> state otherwise.
+   \<^item> The rebalancing is in a valid state (Defined in theory \<open>States\<close>)
+   \<^item> The two ends of the deque are in a size window, such that after finishing the rebalancing the invariant of the \<open>idle\<close> state will be met. 
 
 Functions:
 
  \<^descr> \<open>is_empty\<close>: Checks if a deque is in the \<open>Empty\<close> state
- \<^descr> \<open>deqL’\<close>: Dequeues an element on the left end and return the element and the deque without this element. If the deque is in \<open>idle\<close> state and the size invariant is violated either a \<open>transformation\<close> is started or if there are 3 or less elements left the respective states are used. On \<open>transformation\<close> start, six steps are executed initially. During \<open>transformation\<close> state four steps are executed and if it is finished the deque returns to \<open>idle\<close> state.
+ \<^descr> \<open>deqL’\<close>: Dequeues an element on the left end and return the element and the deque without this element. If the deque is in \<open>idle\<close> state and the size invariant is violated either a \<open>rebalancing\<close> is started or if there are 3 or less elements left the respective states are used. On \<open>rebalancing\<close> start, six steps are executed initially. During \<open>rebalancing\<close> state four steps are executed and if it is finished the deque returns to \<open>idle\<close> state.
  \<^descr> \<open>deqL\<close>: Removes one element on the left end and only returns the new deque.
  \<^descr> \<open>firstL\<close>: Removes one element on the left end and only returns the element.
- \<^descr> \<open>enqL\<close>: Enqueues an element on the left and returns the resulting deque. Like in \<open>deqL'\<close> when violating the size invariant in \<open>idle\<close> state, a \<open>transformation\<close> with six initial steps is started. During \<open>transformation\<close> state four steps are executed and if it is finished the deque returns to \<open>idle\<close> state.
+ \<^descr> \<open>enqL\<close>: Enqueues an element on the left and returns the resulting deque. Like in \<open>deqL'\<close> when violating the size invariant in \<open>idle\<close> state, a \<open>rebalancing\<close> with six initial steps is started. During \<open>rebalancing\<close> state four steps are executed and if it is finished the deque returns to \<open>idle\<close> state.
  \<^descr> \<open>swap\<close>: The two ends of the deque are swapped.
  \<^descr> \<open>deqR’\<close>, \<open>deqR\<close>, \<open>firstR\<close>, \<open>enqR\<close>: Same behaviour as the left-counterparts. Implemented using the left-counterparts by swapping the deque before and after the operation.
  \<^descr> \<open>listL\<close>, \<open>listR\<close>: Get all elements of the deque in a list starting at the left or right end. They are needed as list abstractions for the correctness proofs.
@@ -38,7 +38,7 @@ datatype 'a deque =
   | Two 'a 'a
   | Three 'a 'a 'a 
   | Idle "'a idle" "'a idle"
-  | Transforming "'a states"
+  | Rebal "'a states"
 
 definition empty where
   "empty = Empty"
@@ -59,8 +59,8 @@ fun swap :: "'a deque \<Rightarrow> 'a deque" where
 | "swap (Two x y) = Two y x"
 | "swap (Three x y z) = Three z y x"
 | "swap (Idle left right) = Idle right left"
-| "swap (Transforming (States Left big small)) = (Transforming (States Right big small))"
-| "swap (Transforming (States Right big small)) = (Transforming (States Left big small))"
+| "swap (Rebal (States Left big small)) = (Rebal (States Right big small))"
+| "swap (Rebal (States Right big small)) = (Rebal (States Left big small))"
 
 fun small_deque :: "'a list \<Rightarrow> 'a list \<Rightarrow> 'a deque" where
   "small_deque []     [] = Empty"
@@ -97,11 +97,11 @@ fun deqL' :: "'a deque \<Rightarrow> 'a * 'a deque" where
       let states = States Left big small in
       let states = (step^^6) states in
       
-      (x, Transforming states)
+      (x, Rebal states)
     else 
       case right of Stack r1 r2 \<Rightarrow> (x, small_deque r1 r2)
   )"
-| "deqL' (Transforming (States Left big small)) = (
+| "deqL' (Rebal (States Left big small)) = (
     let (x, small) = Small.pop small in 
     let states = (step^^4) (States Left big small) in
     case states of 
@@ -109,9 +109,9 @@ fun deqL' :: "'a deque \<Rightarrow> 'a * 'a deque" where
           (Big.Common (Common.Idle _ big))
           (Small.Common (Common.Idle _ small)) 
            \<Rightarrow> (x, Idle small big)
-     | _ \<Rightarrow> (x, Transforming states)
+     | _ \<Rightarrow> (x, Rebal states)
   )"
-| "deqL' (Transforming (States Right big small)) = (
+| "deqL' (Rebal (States Right big small)) = (
     let (x, big) = Big.pop big in 
     let states = (step^^4) (States Right big small) in
     case states of 
@@ -119,7 +119,7 @@ fun deqL' :: "'a deque \<Rightarrow> 'a * 'a deque" where
           (Big.Common (Common.Idle _ big)) 
           (Small.Common (Common.Idle _ small)) \<Rightarrow>
             (x, Idle big small)
-     | _ \<Rightarrow> (x, Transforming states)
+     | _ \<Rightarrow> (x, Rebal states)
   )"
 
 fun deqR' :: "'a deque \<Rightarrow> 'a * 'a deque" where
@@ -160,9 +160,9 @@ fun enqL :: "'a \<Rightarrow> 'a deque \<Rightarrow> 'a deque" where
         let states = States Right big small in
         let states = (step^^6) states in
         
-        Transforming states
+        Rebal states
   )"
-| "enqL x (Transforming (States Left big small)) = (
+| "enqL x (Rebal (States Left big small)) = (
     let small = Small.push x small in 
     let states = (step^^4) (States Left big small) in
     case states of 
@@ -170,9 +170,9 @@ fun enqL :: "'a \<Rightarrow> 'a deque \<Rightarrow> 'a deque" where
           (Big.Common (Common.Idle _ big))
           (Small.Common (Common.Idle _ small)) 
          \<Rightarrow> Idle small big
-     | _ \<Rightarrow> Transforming states
+     | _ \<Rightarrow> Rebal states
   )"
-| "enqL x (Transforming (States Right big small)) = (
+| "enqL x (Rebal (States Right big small)) = (
     let big = Big.push x big in 
     let states = (step^^4) (States Right big small) in
     case states of 
@@ -180,7 +180,7 @@ fun enqL :: "'a \<Rightarrow> 'a deque \<Rightarrow> 'a deque" where
           (Big.Common (Common.Idle _ big)) 
           (Small.Common (Common.Idle _ small)) 
          \<Rightarrow> Idle big small
-     | _ \<Rightarrow> Transforming states
+     | _ \<Rightarrow> Rebal states
   )"
 
 fun enqR :: "'a \<Rightarrow> 'a deque \<Rightarrow> 'a deque" where
